Well-kindedness of Binder types

src/PlutusIR/Semantics/Static/Kinding/Kinding.v
@@ -96,3 +96,24 @@ Proof.
     intros xs ys H_xs.
     induction H_xs; intros H_ys; try econstructor; eauto.
 Qed.
+
+
+(* TODO: there is probably a higher order thing to create stuff like this *)
+Inductive map_wk_e : list (string * ty) -> Prop :=
+  | MW_nil_e :
+      map_wk_e nil
+  | MW_cons_e : forall X Δ T (xs : list (string * ty)) K,
+      map_wk_e xs ->
+      has_kind Δ T K ->
+      map_wk_e ((X, T) :: xs).
+
+(* TODO: Is this what we usually call app? *)
+Lemma map_wk_app_e : forall xs ys,
+  map_wk_e xs ->
+  map_wk_e ys ->
+  map_wk_e (xs ++ ys).
+Proof.
+    intros xs ys H_xs.
+    induction H_xs; intros H_ys; try econstructor; eauto.
+Qed.
+
